compiler/backend/passes/pure_comp_confScript.sml
@@ -8,20 +8,23 @@ val _ = new_theory "pure_comp_conf";
 
 Datatype:
   compiler_opts = <|
-      do_pure_simp  : bool ;  (* pure-to-pure *)
-      do_demands    : bool ;  (* pure-to-pure *)
+      do_pure_sort  : bool ;  (* pure-to-pure binding group analysis *)
+      do_pure_clean : bool ;  (* pure-to-pure cleaning / deadcode elimination *)
+      do_demands    : bool ;  (* demand analysis *)
       do_split_dlam : bool ;  (* thunk-to-thunk *)
       do_app_unit   : bool    (* state-to-state *)
     |>
 End
 
-Overload pure_simp_flag[local] = “strlit "-simp"”
-Overload demands_flag[local]   = “strlit "-demands"”
-Overload dlam_flag[local]      = “strlit "-dlam"”
-Overload unit_flag[local]      = “strlit "-unit"”
+Overload pure_sort_flag[local]  = “strlit "-sort"”
+Overload pure_clean_flag[local] = “strlit "-clean"”
+Overload demands_flag[local]    = “strlit "-demands"”
+Overload dlam_flag[local]       = “strlit "-dlam"”
+Overload unit_flag[local]       = “strlit "-unit"”
 
 Definition all_flags_def:
-  all_flags = [pure_simp_flag;
+  all_flags = [pure_sort_flag;
+               pure_clean_flag;
                demands_flag;
                dlam_flag;
                unit_flag]
@@ -31,10 +34,11 @@ Definition read_cline_args_def:
   read_cline_args (cl:mlstring list) ⇔
     case FILTER (λa. ~MEM a all_flags) cl of
     | (a::_) => INR (concat [strlit "ERROR: unknown flag "; a; strlit "\n"])
-    | [] => INL <| do_pure_simp  := ¬ MEM pure_simp_flag cl ;
-                   do_demands    := ¬ MEM demands_flag cl   ;
-                   do_split_dlam := ¬ MEM dlam_flag cl      ;
-                   do_app_unit   := ¬ MEM unit_flag cl      |>
+    | [] => INL <| do_pure_sort  := ¬ MEM pure_sort_flag cl  ;
+                   do_pure_clean := ¬ MEM pure_clean_flag cl ;
+                   do_demands    := ¬ MEM demands_flag cl    ;
+                   do_split_dlam := ¬ MEM dlam_flag cl       ;
+                   do_app_unit   := ¬ MEM unit_flag cl       |>
 End
 
 val default = EVAL “read_cline_args []” |> concl |> rand |> rand
