compiler/proofs/pure_compilerProofScript.sml
@@ -29,35 +29,57 @@ Theorem compiler_correctness:
          (itree_semantics cake)
 Proof
   strip_tac \\ gvs [compile_to_ast_def,frontend_def,AllCaseEqs()]
-  \\ qabbrev_tac ‘e3 = transform_cexp c e1’
+  \\ qabbrev_tac ‘e4 = transform_cexp c e1’
+  \\ qabbrev_tac ‘e3 = clean_cexp c e4’
   \\ qabbrev_tac ‘e2 = demands_analysis c e3’
-  \\ ‘letrecs_distinct (exp_of e3)’
-     by simp [Abbr ‘e3’, transform_cexp_letrecs_distinct]
+  \\ ‘letrecs_distinct (exp_of e3)’ by (
+      simp[Abbr `e3`, Abbr `e4`] >>
+      irule clean_cexp_letrecs_distinct >> simp[transform_cexp_letrecs_distinct])
   \\ qspec_then ‘e3’ assume_tac demands_analysis_soundness \\ fs []
   \\ gvs[DefnBase.one_line_ify NONE pure_inferenceTheory.to_option_def, AllCaseEqs()]
   \\ drule_then strip_assume_tac infer_types_SOME
   \\ gvs[pure_inferenceTheory.infer_types_def, pure_inferenceTheory.fail_def,
          pure_typingTheory.namespace_init_ok_def, AllCaseEqs()] >>
      drule $ INST_TYPE [alpha |-> ``:(mlstring,unit) map``] infer_top_level_typed >>
-     disch_then $ qspecl_then [`empty`,`e3`] assume_tac >> gvs[] >>
+     disch_then $ qspecl_then [`empty`,`e4`] assume_tac >> gvs[] >>
+     `cexp_wf e3 ∧ NestedCase_free e3 ∧
+      type_tcexp (append_ns initial_namespace ns') 0 [] [] (tcexp_of e3) (M Unit)` by (
+        gvs[pure_letrec_cexpTheory.clean_cexp_def] >> FULL_CASE_TAC >> gvs[Abbr `e3`] >>
+        irule_at Any clean_all_cexp_cexp_wf >> simp[] >>
+        drule_all clean_all_preserves_typing >> rw[] >>
+        irule pure_typingPropsTheory.type_tcexp_NestedCase_free >> simp[SF SFY_ss]) >>
      `cexp_wf e2 ∧ NestedCase_free e2 ∧
-      type_tcexp (append_ns initial_namespace ns') 0 [] [] (tcexp_of e2) (M Unit)` by (
+      type_tcexp (append_ns initial_namespace ns') 0 [] [] (tcexp_of e2) (M Unit)`
+      by (
         gvs[pure_demands_analysisTheory.demands_analysis_def] >>
         FULL_CASE_TAC >> gvs[] >>
         qabbrev_tac `d = demands_analysis_fun Nil e3 (empty str_compare)` >>
         PairCases_on `d` >> gvs[] >>
         dxrule_then assume_tac $ cj 5 demands_analysis_fun_insert_seq >> gvs[] >>
-        dxrule_all_then assume_tac pure_typingPropsTheory.insert_seq_imps >> gvs[]) >>
+        dxrule_all_then assume_tac pure_typingPropsTheory.insert_seq_imps >> gvs[]
+        ) >>
      dxrule well_typed_program_imps >> simp[] >>
      impl_tac >- gvs[pure_tcexp_lemmasTheory.cexp_wf_tcexp_wf] >> strip_tac
-  \\ qsuff_tac ‘itree_of (exp_of e3) = itree_of (exp_of e2)’
+  \\ qsuff_tac ‘itree_of (exp_of e4) = itree_of (exp_of e2)’
   >- (
     disch_then $ rewrite_tac o single \\ simp[]
     \\ irule_at Any pure_to_cakeProofTheory.pure_to_cake_correct
     \\ fs [cns_ok_def, pure_typingTheory.namespace_init_ok_def, EXISTS_PROD]
-    )
-  \\ mp_tac safe_exp_app_bisim_F_IMP_same_itree
-  \\ gvs [pure_exp_relTheory.app_bisimilarity_eq]
+    ) >>
+  qspec_then `e4` mp_tac clean_cexp_correct >> strip_tac >>
+  dxrule_at Any $ iffRL pure_exp_relTheory.app_bisimilarity_eq >> simp[] >> impl_tac
+  >- (
+    imp_res_tac pure_typingPropsTheory.type_tcexp_freevars_tcexp >>
+    gvs[pure_tcexp_lemmasTheory.freevars_tcexp_of,
+        pure_cexp_lemmasTheory.freevars_exp_of, pure_expTheory.closed_def]
+    ) >>
+  strip_tac >> dxrule bisimilarity_IMP_semantics_eq >>
+  rw[GSYM pure_semanticsTheory.itree_of_def] >>
+  irule safe_exp_app_bisim_F_IMP_same_itree >> gvs[] >>
+  irule $ iffRL pure_exp_relTheory.app_bisimilarity_eq >> gvs[] >>
+  imp_res_tac pure_typingPropsTheory.type_tcexp_freevars_tcexp >>
+  gvs[pure_tcexp_lemmasTheory.freevars_tcexp_of,
+      pure_cexp_lemmasTheory.freevars_exp_of, pure_expTheory.closed_def]
 QED
 
 Theorem alternative_compiler_correctness:
@@ -110,47 +132,19 @@ Theorem pure_compiler_to_string_correct:
        (itree_of (exp_of pure_ce))
        (itree_semantics cake_prog)
 Proof
-  strip_tac \\ gvs [compile_def,AllCaseEqs()]
-  \\ fs [string_to_ast_ast_to_string]
-  \\ qabbrev_tac ‘e3 = transform_cexp c e1’
-  \\ qabbrev_tac ‘e2 = demands_analysis c e3’
-  \\ ‘letrecs_distinct (exp_of e3)’
-     by simp [Abbr ‘e3’, transform_cexp_letrecs_distinct]
-  \\ qspec_then ‘e3’ assume_tac demands_analysis_soundness \\ fs []
-  \\ gvs[DefnBase.one_line_ify NONE pure_inferenceTheory.to_option_def, AllCaseEqs()]
-  \\ drule_then strip_assume_tac infer_types_SOME
-  \\ gvs[pure_inferenceTheory.infer_types_def, pure_inferenceTheory.fail_def,
-         pure_typingTheory.namespace_init_ok_def, AllCaseEqs()] >>
-     drule $ INST_TYPE [alpha |-> ``:(mlstring,unit) map``] infer_top_level_typed >>
-     disch_then $ qspecl_then [`empty`,`e3`] assume_tac >> gvs[] >>
-     `cexp_wf e2 ∧ NestedCase_free e2 ∧
-      type_tcexp (append_ns initial_namespace ns') 0 [] [] (tcexp_of e2) (M Unit)` by (
-        gvs[pure_demands_analysisTheory.demands_analysis_def] >>
-        FULL_CASE_TAC >> gvs[] >>
-        qabbrev_tac `d = demands_analysis_fun Nil e3 (empty str_compare)` >>
-        PairCases_on `d` >> gvs[] >>
-        dxrule_then assume_tac $ cj 5 demands_analysis_fun_insert_seq >> gvs[] >>
-        dxrule_all_then assume_tac pure_typingPropsTheory.insert_seq_imps >> gvs[]) >>
-     dxrule well_typed_program_imps >> simp[] >>
-     impl_tac >- gvs[pure_tcexp_lemmasTheory.cexp_wf_tcexp_wf] >> strip_tac
-  \\ qsuff_tac ‘itree_of (exp_of e1) = itree_of (exp_of e2)’
+  rw[compile_to_string] >> simp[string_to_ast_ast_to_string] >>
+  drule compiler_correctness >> rw[] >> gvs[frontend_def, AllCaseEqs()] >>
+  qspec_then `e1` assume_tac transform_cexp_correct >>
+  drule_at Any $ iffRL pure_exp_relTheory.app_bisimilarity_eq >> reverse impl_tac
   >- (
-    disch_then $ rewrite_tac o single
-    \\ irule_at Any pure_to_cakeProofTheory.pure_to_cake_correct
-    \\ fs [cns_ok_def, pure_typingTheory.namespace_init_ok_def, EXISTS_PROD]
-    )
-  \\ mp_tac safe_exp_app_bisim_F_IMP_same_itree
-  \\ gvs [pure_exp_relTheory.app_bisimilarity_eq]
-  \\ disch_then drule_all \\ fs []
-  \\ qspec_then ‘e1’ mp_tac transform_cexp_correct
-  \\ gvs [] \\ rpt strip_tac
-  \\ mp_tac bisimilarity_IMP_semantics_eq
-  \\ gvs [pure_exp_relTheory.app_bisimilarity_eq,GSYM pure_semanticsTheory.itree_of_def]
-  \\ disch_then drule \\ fs []
-  \\ disch_then irule
-  \\ simp[pure_expTheory.closed_def, pure_cexp_lemmasTheory.freevars_exp_of]
-  \\ gvs[string_to_cexp_def] \\ pairarg_tac \\ gvs[]
-  \\ drule_at Any $ iffLR ast_to_cexpTheory.closed_under \\ simp[]
+    rw[] >> drule bisimilarity_IMP_semantics_eq >>
+    simp[GSYM pure_semanticsTheory.itree_of_def]
+    ) >>
+  gvs[DefnBase.one_line_ify NONE pure_inferenceTheory.to_option_def, AllCaseEqs()] >>
+  drule infer_types_SOME >> strip_tac >>
+  gvs[string_to_cexp_def] >> pairarg_tac >> gvs[] >>
+  drule_at Any $ iffLR ast_to_cexpTheory.closed_under >>
+  simp[pure_expTheory.closed_def, pure_cexp_lemmasTheory.freevars_exp_of]
 QED
 
 val _ = export_theory();
