compiler/pure_compilerScript.sml
@@ -35,9 +35,11 @@ Definition compile_def:
         case to_option i of
         | NONE => NONE
         | SOME _ =>
-          let e3 = demands_analysis c e2 in
+          let e3 = clean_cexp c e2 in
+          let _ = empty_ffi (strlit "clean_cexp") in
+          let e4 = demands_analysis c e3 in
           let _ = empty_ffi (strlit "demands_analysis") in
-            SOME (ast_to_string $ pure_to_cake c ns e3)
+            SOME (ast_to_string $ pure_to_cake c ns e4)
 End
 
 Definition compile_to_ast_def:
@@ -50,8 +52,9 @@ Definition compile_to_ast_def:
         case to_option i of
         | NONE => NONE
         | SOME _ =>
-          let e3 = demands_analysis c e2 in
-          SOME (pure_to_cake c ns e3)
+          let e3 = clean_cexp c e2 in
+          let e4 = demands_analysis c e3 in
+          SOME (pure_to_cake c ns e4)
 End
 
 (********** Alternative phrasings **********)
@@ -62,8 +65,9 @@ Theorem compile_monadically:
     (e1,ns) <- string_to_cexp s ;
     e2 <<- transform_cexp c e1 ;
     to_option $ infer_types ns e2 ;
-    e3 <<- demands_analysis c e2 ;
-    return (ast_to_string $ pure_to_cake c ns e3)
+    e3 <<- clean_cexp c e2 ;
+    e4 <<- demands_analysis c e3 ;
+    return (ast_to_string $ pure_to_cake c ns e4)
   od
 Proof
   simp[compile_def] >> EVERY_CASE_TAC >> simp[]
@@ -93,8 +97,9 @@ Theorem compile_to_ast_alt_def:
     case frontend c s of
     | NONE => NONE
     | SOME (e2,ns) =>
-        let e3 = demands_analysis c e2 in
-        SOME (pure_to_cake c ns e3)
+        let e3 = clean_cexp c e2 in
+        let e4 = demands_analysis c e3 in
+        SOME (pure_to_cake c ns e4)
 Proof
   rw[compile_to_ast_def, frontend_def] >>
   rpt (TOP_CASE_TAC >> simp[])
